examples/graph/module-edits/Data/Graph/Inductive/Graph/midamble.v
@@ -1,76 +1,113 @@
 Definition ulabNodes  {a} l :=
   map (fun (x: Node * a) => let (i, l):= x in i) l.
 
-Definition ulabNodes_gr {gr} `{(Graph gr)} {a} {b} (g: gr a b) :=
+Definition nodeList {gr} `{(Graph gr)} {a} {b} (g: gr a b) : list Node :=
   ulabNodes (labNodes g).
 
 Definition ulabEdges {b} l :=
   map (fun (x: Node * Node * b) => match x with |  (u, v, l) => (u,v) end) l.
 
-Definition ulabEdges_gr {gr : Type -> Type -> Type}  {a b : Type} `{(Graph gr)} (g: gr a b) :=
+Definition edgeList {gr : Type -> Type -> Type}  {a b : Type} `{(Graph gr)} (g: gr a b) : list Edge :=
   ulabEdges (labEdges g).
 
-(*We want a specification of a graph*)
+Definition mem {A: Type} (x: A) (l: list A)  (H: (forall x y:A, {x = y} + {x <> y}))  : bool :=
+  if (in_dec H x l) then true else false.
 
-(*Find a vertex in a graph*)
-Definition vIn {gr a b} `{Graph gr} (g: gr a b) (v: Node) : Prop :=
-  In v (ulabNodes_gr g).
+Definition vIn {gr a b} `{Graph gr} (g: gr a b) (v: Node) : bool :=
+  mem v (nodeList g) N.eq_dec.
 
-(*Find an edge in a graph*)
-Definition eIn {gr a b} `{Graph gr} (g: gr a b) (u v: Node) : Prop :=
-  In (u,v) (ulabEdges_gr g).
+Lemma pair_dec: forall {a b : Type},
+  (forall x y : a, {x = y} + { x <> y}) ->
+  (forall x y : b, {x = y} + {x <> y}) ->
+  (forall x y : (a * b), {x = y} + { x <> y}).
+Proof.
+  intros. destruct x. destruct y. specialize (X a0 a1). specialize (X0 b0 b1).
+  destruct X. subst. destruct X0. subst. left. reflexivity. right. intro. inversion H; subst; contradiction.
+  right. intro. inversion H; subst; contradiction.
+Qed.
 
-Definition Desc {gr a b} `{Graph gr} (g: gr a b) (sz: GHC.Num.Int) fv fe: Prop :=
-  forall (P: (gr a b) -> Prop),
-  (forall g',
-    noNodes g' =  sz ->
-    (forall (v: Node), vIn g' v <-> fv v) -> 
-    (forall (u v : Node), eIn g' u v <-> fe u v) ->
-  P g') -> P g.
+Definition eIn {gr a b} `{Graph gr} (g: gr a b) (u v : Node) : bool :=
+  mem (u,v) (edgeList g) (pair_dec N.eq_dec N.eq_dec).
 
-
-(*Should replace Int with Nat here in noNodes bc it is the length of a list
-TODO: see if replacing with a nat is ok or if it should be BinNumsN - we define as length of list,
-so should be nat, but ok if have to change - just need things to be aligned*)
-Class LawfulGraph (gr: Type  -> Type -> Type) `{Graph gr} := {
-  empty_def: forall (a b : Type), Desc (@empty gr _ a b) #0 (fun v => False) (fun u v => False);
-  is_empty_def: forall (a b: Type) (g: gr a b), isEmpty g = true <-> Desc g #0 (fun v => False) (fun u v => False);
-  (*If the vertex is in the graph, then we can get a context with the vertex we queried, and every predecessor
-    is an edge (u', v), while every successor is an edge (v, u') *)
-  match_1: forall (a b : Type) (g: gr a b) v, vIn g v -> 
-    exists i x l o g', @match_ gr _ a b v g = (Some (i, x, l, o), g') /\ x = v /\ 
-    (forall u' l', In (l',u') i -> eIn g u' v) /\ (forall u' l', In (l',u') o -> eIn g v u');
-  (*The remaining graph has the same vertices and edges as the previous graph, except for v and its neighbors*)
-  match_2: forall (a b : Type) (g: gr a b) v x g' n, vIn g v -> @match_ gr _ a b v g = (Some x, g') ->
-    (noNodes g) = BinInt.Z.of_nat (S n) ->
-    Desc g' (BinInt.Z.of_nat n) (fun u => vIn g u /\ u <> v) (fun x y => eIn g x y /\ x <> v /\ y <> v);
-  (*See if I need this specifically*)
-  match_3: forall (a b : Type) (g: gr a b) v x g', match_ v g = (Some x, g') -> vIn g v;
-  (*Also see if I need this*)
-  match_4: forall (a b : Type) (g : gr a b) v n g' i l o, match_ v g = (Some (i, n, l, o), g') -> v = n;
-  mkGraph_def: forall (a b : Type) lv le, Desc (mkGraph lv le) (BinInt.Z.of_nat (@length (LNode a) lv))
-     (fun v => In v (@ulabNodes a lv))
-     (fun u v => In (u,v) (@ulabEdges b le));
-  matchAny_def: forall (a b : Type) (g: gr a b) g' x i l o, isEmpty g = false ->
-    matchAny g = ((i, x, l, o), g') ->
-    match_ x g = (Some (i, x, l, o), g');
-  noNodes_def: forall (a b : Type) (g: gr a b), noNodes g = BinInt.Z.of_nat (length (labNodes g))
-  (*TODO: others later, see about translating definitions*)
+(*A well formed graph: every function behaves as specified. This may not play too well with graphs with
+  multiple edges between nodes.*)
+Class LawfulGraph (gr: Type -> Type -> Type) `{Graph gr} := {
+  (*Every edge consists of vertices in the graph*)
+  edges_valid: forall {a b : Type} (g: gr a b) (u v : Node), eIn g u v = true ->
+    vIn g u = true /\ vIn g v = true;
+  (*No duplicate vertices (some of the functions have undefined behavior if this is not true)*)
+  vertices_valid: forall {a b: Type} (g: gr a b), NoDup (nodeList g);
+  (*The empty graph has no vertices*)
+  empty_def: forall {a b : Type} (v: Node), vIn (@empty gr _ a b) v = false;
+  (*A graph is empty iff it has no vertices*)
+  isEmpty_def: forall {a b: Type} (g: gr a b) (v: Node), isEmpty g = true <-> (forall v, vIn g v = false);
+  (*Match finds a context iff a vertex is in the graph*)
+  match_in: forall {a b : Type} (g: gr a b) (v : Node), (exists c g', match_ v g = (Some c, g')) <-> vIn g v = true;
+  (*The context for 'match' - NOTE: doesn't play well with multiple edges between nodes, see about this*)  
+  match_context: forall {a b : Type} (g: gr a b) (v: Node) i x l o g',
+    match_ v g = (Some (i, x, l, o), g') -> v = x /\ 
+    (forall y, In y (map snd i) <-> eIn g y v = true) /\
+    (forall y, In y (map snd o) <-> eIn g v y = true);
+  (*The rest of the graph for a match*)
+  match_remain_some: forall {a b: Type} (g: gr a b) (v: Node) c g',
+    match_ v g = (Some c, g') -> 
+    (forall u, vIn g' u = true <-> vIn g u = true /\ u <> v) /\
+    (forall x y, eIn g' x y = true <-> eIn g x y = true /\ x <> v /\ y <> v);
+  (*This is true in the STArray and IOArray implementations, and makes things much simpler*)
+  match_remain_none: forall {a b: Type} (g: gr a b) (v: Node) g',
+    match_ v g = (None, g') ->
+    g = g';
+  (*matchAny gives a match_ for some vertex in the graph*)
+  matchAny_def: forall {a b: Type} (g: gr a b),
+    isEmpty g = false ->
+    exists v i l o g', matchAny g = ((i, v, l, o), g') /\ vIn g v = true /\
+    match_ v g = (Some (i, v, l, o), g');
+  (*noNodes is number of nodes in list (another reason why no duplicates is important)*)
+  noNodes_def: forall {a b: Type} (g: gr a b),
+    Z.abs_nat (noNodes g) = length (labNodes g)
 }.
+
+(*It turns out to be very annoying to prove that match_ decreases the size of the graph. The easiest way
+  found is to prove that the new vertex list along with the vertex is a permutation of the original list,
+  and so has the same length. We need to prove an auxiliary lemma first.*)
+Lemma perm_remove: forall {A: Type} (l l': list A)(x : A),
+  (forall (x y : A), {x = y} + { x <> y}) ->
+  In x l' ->
+  (forall y, In y l <-> In y l' /\ y <> x) ->
+  NoDup l ->
+  NoDup l' ->
+  Permutation l' (x :: l).
+Proof.
+  intros. assert (forall y, In y l' <-> In y (x :: l)). { simpl. split; intros.
+  destruct (X x y). left. assumption. right. rewrite H0. split. assumption. auto.
+  destruct H3. subst. assumption. apply H0 in H3. intuition. }
+  assert (~In x l). intro. rewrite H0 in H4. destruct H4. contradiction.
+  assert (NoDup (x :: l)). constructor. assumption. assumption.
+  apply NoDup_Permutation. assumption. assumption. apply H3.
+Qed.
 
 Lemma match_decr_size: forall {a b : Type} {gr} `{Graph gr} `{LawfulGraph gr} c g' (g: gr a b) v,
   (Some c, g') = match_ v g ->
   BinInt.Z.abs_nat (noNodes g') < BinInt.Z.abs_nat (noNodes g).
 Proof.
-  intros. symmetry in H2. destruct c. destruct p. destruct p. 
-  assert (vIn g v). eapply match_3. apply H2.
-  pose proof (noNodes_def _ _ g). assert (length (labNodes g) > 0).
-  destruct (length (labNodes g)) eqn : A.
-  apply length_zero_iff_nil in A. unfold vIn in H3. unfold ulabNodes_gr in H3. rewrite A in H3.
-  destruct H3. omega. destruct (length (labNodes g)) eqn : B. omega.
-  assert (v = n) by (eapply match_4; apply H2); subst.
-  apply (match_2 a b g n (a2, n, a1, a0) g' n0). assumption. assumption. assumption. intros.
-  rewrite !noNodes_def in *.  rewrite Zabs2Nat.id. rewrite Zabs2Nat.id. omega.
+  intros. rewrite noNodes_def. rewrite noNodes_def. 
+  pose proof (vertices_valid g'). 
+  assert (length (labNodes g') = length(nodeList g')). unfold nodeList. unfold ulabNodes.
+  rewrite map_length. reflexivity. rewrite H4. clear H4. assert (length (labNodes g) = length (nodeList g)).
+  unfold nodeList. unfold ulabNodes. rewrite map_length. reflexivity. rewrite H4. clear H4.
+   symmetry in H2.
+  pose proof (match_remain_some g v c g' H2). destruct H4. clear H5.
+  assert (forall u, In u (nodeList g') <-> In u (nodeList g) /\ u <> v). { intros.
+  specialize (H4 u). unfold vIn in H4. unfold mem in H4.
+  assert (forall l x, ((if in_dec N.eq_dec x l then true else false) = true) <-> In x l). {
+  intros. destruct (in_dec N.eq_dec x l). split; intros; try(assumption); try(reflexivity).
+  split; intros. inversion H5. contradiction. } rewrite H5 in H4. rewrite H5 in H4.
+  apply H4. } pose proof (vertices_valid g). pose proof (match_in g v).
+  assert (In v (nodeList g)). assert (vIn g v = true). apply H7. exists c. exists g'.
+  assumption. unfold vIn in H8. unfold mem in H8.
+  match goal with | [H: (if ?x then _ else _) = _ |- _] => destruct x end.
+  assumption. inversion H8. pose proof (perm_remove (nodeList g') (nodeList g) v N.eq_dec H8 H5 H3 H6).
+  apply Permutation_length in H9. simpl in H9. omega.
 Qed.
 
 Lemma matchAny_decr_size: forall {a b : Type} {gr} `{Graph gr} `{LawfulGraph gr} c g' (g: gr a b),
@@ -78,6 +115,9 @@ Lemma matchAny_decr_size: forall {a b : Type} {gr} `{Graph gr} `{LawfulGraph gr}
   isEmpty g = false ->
   BinInt.Z.abs_nat (noNodes g') < BinInt.Z.abs_nat (noNodes g).
 Proof.
-  intros. symmetry in H2. destruct c. destruct p. destruct p. 
-  apply (matchAny_def _ _ _ _ _ _ _ _ H3) in H2. symmetry in H2. eapply match_decr_size; apply H2.
+  intros. symmetry in H2. destruct c. destruct p. destruct p. pose proof (matchAny_def g H3).
+  repeat (match goal with | [H: exists _, _ |- _] => destruct H | [H: ?x /\ ?y |- _] => destruct H end).
+  symmetry in H6.
+  rewrite H4 in H2. inversion H2; subst.
+  apply (match_decr_size (a2, n, a1, a0) g' g n H6).
 Qed.
